## Пункт а)

$$ f(x) = 3x - x^3 $$

$$ f(-x) = -3x + x^3 = -(3x - x^3) = -f(x) $$

Значит, $f(x)$ — нечетная функция.

## Пункт б)

$$ f(x) = \sqrt[3]{(1-x)^2} + \sqrt[3]{(1+x)^2} $$

$$ f(-x) = \sqrt[3]{(1-(-x))^2} + \sqrt[3]{(1+(-x))^2} = \\[5px] = \sqrt[3]{(1+x)^2} + \sqrt[3]{(1-x)^2} = f(x) $$

Значит, $f(x)$ — четная функция.

## Пункт в)

$$ f(x) = a^x + a^{-x} \quad (a>0) $$

$$ f(-x) = a^{-x} + a^{-(-x)} = a^{x} + a^{-x} = f(x) $$

Значит, $f(x)$ — четная функция.

## Пункт г)

$$ f(x) = \ln\frac{1-x}{1+x} $$

$$ f(-x) = \ln\frac{1-(-x)}{1+(-x)} = \ln\frac{1+x}{1-x} = \ln\left(\frac{1-x}{1+x}\right)^{-1} = \\[5px] = -\ln\frac{1-x}{1+x} = -f(x) $$

Значит, $f(x)$ — нечетная функция.

## Пункт д)

$$ f(x) = \ln (x+\sqrt{1+x^2}) $$

$$ f(-x) = \ln(-x+\sqrt{1+(-1)^2 x^2}) = \\[5px] = \ln\left[\frac{(-x+\sqrt{1+x^2})(-x-\sqrt{1+x^2})}{-x-\sqrt{1+x^2}}\right] = \\[5px] = \ln\left( \frac{x^2 - 1 - x^2}{-x-\sqrt{1+x^2}} \right) = \ln\left( \frac{1}{x+\sqrt{1+x^2}} \right) = \\[5px] = \ln (x+\sqrt{1+x^2})^{-1} = -\ln(x^2 + \sqrt{1+x^2}) = -f(x) $$

Значит, $f(x)$ — нечетная функция.