## Пункт а)

$$ f(x) = ax + b \\ f(x+h) = a(x+h) + b = ax + ah + b $$

Поэтому

$$ \varphi(x) = \frac{ax + ah + b - ax - b}{h} = \frac{ah}{h} = a $$

$$ \varphi(x) = a $$

## Пункт б)

$$ f(x) = x^2 \\ f(x+h) = (x+h)^2 = x^2 + 2xh + h^2 $$

Поэтому

$$ \varphi(x) = \frac{x^2 + 2xh + h^2 - x^2}{h} = \frac{2xh + h^2}{h} = 2x + h $$

$$ \varphi(x) = 2x + h $$

## Пункт в)

$$ f(x) = a^x \\ f(x+h) = a^{x+h} = a^x a^h $$

Поэтому

$$ \varphi(x) = \frac{a^x a^h - a^x}{h} = a^x \left(\frac{a^h - 1}{h}\right) $$

$$ \varphi(x) = a^x\left(\frac{a^h - 1}{h}\right) $$